>[!THEOREM] Theorem: Multiplication with the Additive Identity
>Multiplying any element $\alpha$ of a [field](Field.md) $(F,+,\cdot)$ with its additive identity $0$ results in the additive identity.
>
>$$\alpha \cdot 0 = 0 \qquad \forall \alpha \in F$$
>
>>[!PROOF]-
>>$$\alpha \cdot 0 = \alpha \cdot (0 + 0) = \alpha\cdot 0 + \alpha\cdot 0$$
>>$$\alpha \cdot 0 = \alpha \cdot 0 + \alpha \cdot 0$$
>>$$(\alpha \cdot 0) + (-\alpha \cdot 0) = (\alpha \cdot 0) + (\alpha \cdot 0) + (-\alpha \cdot 0)$$
>>$$0 = \alpha \cdot 0$$